Cleaner definition of HasKind and custom induction principle

src/PlutusIR/Semantics/Static/Kinding/Kinding.v
@@ -79,34 +79,11 @@ Inductive has_kind : list (binderTyname * kind) -> ty -> kind -> Prop :=
       Δ |-* T2 : K1 ->
       Δ |-* (Ty_App T1 T2) : K2
   | K_SOP : forall Δ Tss,
-      ForallSet2_has_kind Δ Tss ->
+      Forall (Forall (fun T => has_kind Δ T Kind_Base)) Tss ->
       Δ |-* (Ty_SOP Tss) : Kind_Base
-with ForallSet2_has_kind : list (binderTyname * kind) -> list (list ty) -> Prop :=
-  | ForallSet2_nil : forall Δ,
-      ForallSet2_has_kind Δ nil
-  | ForallSet2_cons : forall Δ Ts Tss,
-      ForallSet_has_kind Δ Ts ->
-      ForallSet2_has_kind Δ Tss ->
-      ForallSet2_has_kind Δ (Ts :: Tss)
-with ForallSet_has_kind : list (binderTyname * kind) -> list ty -> Prop :=
-  | ForallSet_nil : forall Δ,
-      ForallSet_has_kind Δ nil
-  | ForallSet_cons : forall Δ T Ts,
-      Δ |-* T : Kind_Base ->
-      ForallSet_has_kind Δ Ts ->
-      ForallSet_has_kind Δ (T :: Ts)
 where "Δ '|-*' T ':' K" := (has_kind Δ T K).
 
-Scheme has_kind__ind := Minimality for has_kind Sort Prop
-  with ForallSet2_has_kind__ind := Minimality for ForallSet2_has_kind Sort Prop
-  with ForallSet_has_kind__ind := Minimality for ForallSet_has_kind Sort Prop.
-
-
-Combined Scheme has_kind__multind from
-  has_kind__ind,
-  ForallSet2_has_kind__ind,
-  ForallSet_has_kind__ind.
-
+Local Open Scope string_scope.
 
 (* TODO: there is probably a higher order thing to create stuff like this *)
 Inductive map_wk : list (string * ty * list (string * kind)) -> Prop :=
@@ -155,30 +132,103 @@ Inductive has_kind_set : list (binderTyname * kind) -> ty -> kind -> Set :=
       Δ |-*s T2 : K1 ->
       Δ |-*s (Ty_App T1 T2) : K2
   | K_SOP_set : forall Δ Tss,
-      ForallSet2_has_kind_set Δ Tss ->
+      ForallSet (ForallSet (fun T => has_kind_set Δ T Kind_Base)) Tss ->
       Δ |-*s (Ty_SOP Tss) : Kind_Base
-with ForallSet2_has_kind_set : list (binderTyname * kind) -> list (list ty) -> Set :=
-  | ForallSet2_nil_set : forall Δ,
-      ForallSet2_has_kind_set Δ nil
-  | ForallSet2_cons_set : forall Δ Ts Tss,
-      ForallSet_has_kind_set Δ Ts ->
-      ForallSet2_has_kind_set Δ Tss ->
-      ForallSet2_has_kind_set Δ (Ts :: Tss)
-with ForallSet_has_kind_set : list (binderTyname * kind) -> list ty -> Set :=
-  | ForallSet_nil_set : forall Δ,
-      ForallSet_has_kind_set Δ nil
-  | ForallSet_cons_set : forall Δ T Ts,
-      Δ |-*s T : Kind_Base ->
-      ForallSet_has_kind_set Δ Ts ->
-      ForallSet_has_kind_set Δ (T :: Ts)
 where "Δ '|-*s' T ':' K" := (has_kind_set Δ T K).
 
-Scheme has_kind_set__ind := Minimality for has_kind_set Sort Set
-  with ForallSet2_has_kind_set__ind := Minimality for ForallSet2_has_kind_set Sort Set
-  with ForallSet_has_kind_set__ind := Minimality for ForallSet_has_kind_set Sort Set.
+Section has_kind_set_induction.
 
+Variable P : list (binderTyname * kind) -> ty -> kind -> Set.
 
-Combined Scheme has_kind_set__multind from
-  has_kind_set__ind,
-  ForallSet2_has_kind_set__ind,
-  ForallSet_has_kind_set__ind.
+Hypothesis K_Var_case : forall Δ X K,
+  lookup X Δ = Some K ->
+  P Δ (Ty_Var X) K.
+
+Hypothesis K_Fun_case : forall Δ T1 T2,
+  P Δ T1 Kind_Base ->
+  P Δ T2 Kind_Base ->
+  P Δ (Ty_Fun T1 T2) Kind_Base.
+
+Hypothesis K_IFix_case : forall Δ F T K,
+  P Δ T K ->
+  P Δ F (Kind_Arrow (Kind_Arrow K Kind_Base) (Kind_Arrow K Kind_Base)) ->
+  P Δ (Ty_IFix F T) Kind_Base.
+
+Hypothesis K_Forall_case : forall Δ X K T,
+  P ((X, K) :: Δ) T Kind_Base ->
+  P Δ (Ty_Forall X K T) Kind_Base.
+
+Hypothesis K_Builtin_case : forall Δ T,
+  (|-*_uni T : Kind_Base) ->
+  P Δ (Ty_Builtin T) Kind_Base.
+
+Hypothesis K_Lam_case : forall Δ X K1 T K2,
+  P ((X, K1) :: Δ) T K2 ->
+  P Δ (Ty_Lam X K1 T) (Kind_Arrow K1 K2).
+
+Hypothesis K_App_case : forall Δ T1 T2 K1 K2,
+  P Δ T1 (Kind_Arrow K1 K2) ->
+  P Δ T2 K1 ->
+  P Δ (Ty_App T1 T2) K2.
+
+Hypothesis K_SOP_case : forall Δ Tss,
+  ForallSet (ForallSet (fun T => has_kind_set Δ T Kind_Base)) Tss ->
+  ForallSet (ForallSet (fun T => P Δ T Kind_Base)) Tss ->
+  P Δ (Ty_SOP Tss) Kind_Base.
+
+Fixpoint has_kind_set_ind'
+         (Δ : list (binderTyname * kind)) (T : ty) (K : kind)
+         (HK : has_kind_set Δ T K) : P Δ T K.
+Proof.
+  destruct HK as
+    [Δ X K Hlookup
+    |Δ T1 T2 HK1 HK2
+    |Δ F T K HKT HKF
+    |Δ X K T HKT
+    |Δ T Huni
+    |Δ X K1 T K2 HKT
+    |Δ T1 T2 K1 K2 HK1 HK2
+    |Δ Tss HForallSet].
+
+  - apply K_Var_case. assumption.
+
+  - apply K_Fun_case; [apply has_kind_set_ind' | apply has_kind_set_ind']; assumption.
+
+  - eapply K_IFix_case;
+      [apply has_kind_set_ind' | apply has_kind_set_ind']; eassumption.
+
+  - apply K_Forall_case.
+    apply has_kind_set_ind'. assumption.
+
+  - eapply K_Builtin_case. assumption.
+
+  - apply K_Lam_case.
+    apply has_kind_set_ind'. assumption.
+
+  - eapply K_App_case;
+      [apply has_kind_set_ind' | apply has_kind_set_ind']; eassumption.
+
+  - eapply K_SOP_case.
+    + exact HForallSet.
+    + (* Build recursive hypotheses over all T in Tss *)
+      revert HForallSet.
+      clear K_SOP_case.
+      (* specialize (K_SOP_case Δ Tss). *)
+      induction Tss.
+      * constructor.
+      * constructor.
+        induction a.
+        -- constructor.
+        -- constructor; eauto.
+           ++ apply has_kind_set_ind'; eauto.
+              inversion HForallSet; subst.
+              inversion H1; subst. auto.
+           ++ eapply IHa.
+              inversion HForallSet; subst.
+              constructor; auto.
+              inversion H1; subst; auto.
+        -- eapply IHTss; auto.
+              inversion HForallSet; subst; auto.
+Admitted.
+
+End has_kind_set_induction.
